vera/EquivalenceTop.v
@@ -1,4 +1,6 @@
-From vera Require Import Verilog.
+From vera Require Verilog.
+Import Verilog.Verilog.
+Import Verilog.Notations.
 From vera Require Import Variables.
 From vera Require VerilogSemantics.
 Import VerilogSemantics.Sort.
@@ -10,6 +12,7 @@ From vera Require VerilogEquivalence.
 From vera Require Import Common.
 From vera Require Import VerilogSemantics.
 From vera Require Import Tactics.
+From vera Require Import Decidable.
 Import CombinationalOnly.
 Import DefinedEquivalence.
 Import ExactEquivalence.
@@ -18,6 +21,7 @@ From ExtLib Require Import Structures.Monads.
 
 From Stdlib Require Import String.
 From Stdlib Require Import Sorting.Permutation.
+From Stdlib Require Import ProofIrrelevance.
 
 From Equations Require Import Equations.
 
@@ -29,29 +33,33 @@ Local Open Scope verilog_scope.
 Module Pass.
   Record t := Mk {
     pass_name : string;
-    pass_apply :> Verilog.vmodule -> string + Verilog.vmodule;
-    pass_correct : forall v1 v2, pass_apply v1 = inr v2 -> v1 ~~~ v2
+    pass_apply : forall [i o], vmodule i o -> string + vmodule i o;
+    pass_correct : forall [i o] (v1 v2 : vmodule i o), pass_apply v1 = inr v2 -> v1 ~~~ v2
   }.
+
+  #[local]
+  Obligation Tactic := intros.
 
   #[program]
   Definition pure
     (name : string)
-    (f : Verilog.vmodule -> Verilog.vmodule)
-    (f_correct : forall v, f v ~~~ v)
+    (f : forall {i o}, vmodule i o -> vmodule i o)
+    (f_correct : forall {i o} (v : vmodule i o), f v ~~~ v)
     : t := {|
       pass_name := name;
-      pass_apply v := ret (f v)
+      pass_apply _ _ v := ret (f v);
     |}.
-  Next Obligation. symmetry. apply f_correct. Qed.
+  Next Obligation. inv H. symmetry. apply f_correct. Qed.
 
   #[program]
   Definition compose (p1 p2 : t) : t := {|
     pass_name := pass_name p1 ++ " ∘ " ++ pass_name p2;
-    pass_apply v :=
+    pass_apply _ _ v :=
       let* v' := pass_apply p1 v in
       pass_apply p2 v'
   |}.
   Next Obligation.
+    simpl in H.
     monad_inv.
     transitivity v.
     - eapply pass_correct. eassumption.
@@ -69,60 +77,44 @@ Infix "∘" := Pass.compose (at level 20, right associativity) : pass_scope.
 Local Open Scope pass.
 
 Section sort.
-  Import Verilog.
   Import SigTNotations.
 
-  Program Definition sort_module_body v
+  Program Definition sort_module_body {i o} (v : vmodule i o)
     : string
       + {
-        sorted : list Verilog.module_item
-        & sort_module_items (LocationSet.of_varset (VarSet.of_list (Verilog.module_inputs v))) (Verilog.modBody v) = Some sorted
+        sorted : list module_item
+        & sort_module_items (LocationSet.of_varset (VarSet.of_list (module_inputs v))) (modBody v) = Some sorted
       } :=
-    match sort_module_items (LocationSet.of_varset (VarSet.of_list (Verilog.module_inputs v))) (Verilog.modBody v) with
+    match sort_module_items (LocationSet.of_varset (VarSet.of_list (module_inputs v))) (modBody v) with
     | None => inl "Module not sortable"
     | Some sorted => inr (sorted; _)
     end.
 
-  Lemma sort_module_body_spec v sorted Hsort :
+  Lemma sort_module_body_spec {i o} (v : vmodule i o) sorted Hsort :
     sort_module_body v = inr (sorted; Hsort) ->
     sort_module_items
-      (LocationSet.of_varset (VarSet.of_list (Verilog.module_inputs v)))
-      (Verilog.modBody v) = Some sorted.
+      (LocationSet.of_varset (VarSet.of_list (module_inputs v)))
+      (modBody v) = Some sorted.
   Proof.
     unfold sort_module_body.
     destruct (sort_module_items
-                (LocationSet.of_varset (VarSet.of_list (Verilog.module_inputs v)))
-                (Verilog.modBody v)) eqn:E;
+                (LocationSet.of_varset (VarSet.of_list (module_inputs v)))
+                (modBody v)) eqn:E;
       intros; congruence.
   Qed.
 
-  Lemma sort_module_body_wf_write_targets v sorted :
-    sort_module_items (LocationSet.of_varset (VarSet.of_list (Verilog.module_inputs v))) (Verilog.modBody v) = Some sorted ->
-    LocationSet.Subset
-      (module_body_writes sorted)
-      (LocationSet.of_varset
-        (VarSet.diff
-           (VarSet.of_list (List.map variable_of_decl (modVariableDecls v)))
-           (VarSet.of_list (inputs_of_decls (modVariableDecls v))))).
-  Proof.
-    intros Hperm.
-    rewrite <- sort_module_items_permutation by eassumption.
-    apply modWfWriteTargets.
-  Qed.
-
-  Definition sort_vmodule (v : Verilog.vmodule) : string + Verilog.vmodule :=
-    traceBracket ("Sort " ++ Verilog.modName v) (
+  #[refine]
+  Definition sort_vmodule {i o} (v : vmodule i o) : string + vmodule i o :=
+    traceBracket ("Sort " ++ modName v) (
       let* (sorted_body; Hsort) := sort_module_body v in
       ret {|
-        Verilog.modName := Verilog.modName v;
-        Verilog.modVariableDecls := Verilog.modVariableDecls v;
-        Verilog.modBody := sorted_body;
-        Verilog.modWfVariablesNoDup := Verilog.modWfVariablesNoDup v;
-        Verilog.modWfWriteTargets := sort_module_body_wf_write_targets v sorted_body Hsort
+        modName := modName v;
+        modBody := sorted_body;
       |}
     ).
+  Proof. all: destruct v; assumption. Defined.
   
-  Theorem sort_vmodule_exact_equivalence v1 v2 :
+  Theorem sort_vmodule_exact_equivalence {i o} (v1 v2 : vmodule i o) :
     sort_vmodule v1 = inr v2 ->
     v1 ~~~ v2.
   Proof.
@@ -131,7 +123,7 @@ Section sort.
     pose proof (sort_module_body_spec _ _ _ E) as Hsort.
     apply equal_exact_equivalence; try reflexivity; expect 1.
     unfold run_vmodule. simpl.
-    unfold Verilog.module_inputs in *; simpl in *.
+    unfold module_inputs in *; simpl in *.
     apply functional_extensionality.
     intros regs. rewrite Hsort.
     rewrite sort_module_items_stable
@@ -141,13 +133,13 @@ Section sort.
 End sort.
 
 Definition sort_vmodule_pass : Pass.t :=
-  Pass.Mk "Sort" sort_vmodule sort_vmodule_exact_equivalence.
+  Pass.Mk "Sort" (@sort_vmodule) (@sort_vmodule_exact_equivalence).
 Definition simpl_vmodule_pass : Pass.t :=
-  Pass.pure "Simpl" simpl_vmodule simpl_vmodule_exact_equivalence.
+  Pass.pure "Simpl" (@simpl_vmodule) (@simpl_vmodule_exact_equivalence).
 Definition break_const_assigns_pass : Pass.t :=
-  Pass.pure "BreakConstAssigns" break_const_assigns_vmodule break_const_assigns_exact_equivalence.
+  Pass.pure "BreakConstAssigns" (@break_const_assigns_vmodule) (@break_const_assigns_exact_equivalence).
 Definition drop_unused_pass : Pass.t :=
-  Pass.Mk "DropUnused" drop_unused drop_unused_exact_equivalence.
+  Pass.Mk "DropUnused" (@drop_unused) (@drop_unused_exact_equivalence).
 
 Definition verilog_pipeline : Pass.t :=
   sort_vmodule_pass
@@ -158,15 +150,31 @@ Definition verilog_pipeline : Pass.t :=
 Definition lower_verilog :=
   Pass.pass_apply verilog_pipeline.
 
-Definition verilog_to_smt_general t verilog : sum string SMTQueries.query :=
-  let* verilog' := verilog_pipeline verilog in
+Import EqNotations.
+
+Definition verilog_to_smt_general {i o} t (verilog : vmodule i o) : sum string SMTQueries.query :=
+  let* verilog' := Pass.pass_apply verilog_pipeline verilog in
   VerilogToSMT.verilog_to_smt t verilog'.
 
-Definition equivalence_query_general (verilog1 verilog2 : Verilog.vmodule) : sum string SMTQueries.query :=
-  let* verilog1' := verilog_pipeline verilog1 in
-  let* verilog2' := verilog_pipeline verilog2 in
+Definition rew_interface {i1 o1 i2 o2} (inputs_eq : i1 = i2) (outputs_eq : o1 = o2) (v : vmodule i1 o1) : vmodule i2 o2 :=
+  rew [fun i : list Var.t => vmodule i o2] inputs_eq in
+  rew [fun o : list Var.t => vmodule i1 o] outputs_eq in v.
 
-  VerilogEquivalence.equivalence_query verilog1' verilog2'.
+Search (_ = rew _ in _).
+
+Lemma rew_interface_refl {i o} (inputs_eq : i = i) (outputs_eq : o = o) (v : vmodule i o) :
+  rew_interface inputs_eq outputs_eq v = v.
+Proof. unfold rew_interface. rewrite <- ! eq_rect_eq. reflexivity. Qed.
+  
+Definition equivalence_query_general {i1 o1 i2 o2} (verilog1 : vmodule i1 o1) (verilog2 : vmodule i2 o2)
+    : sum string SMTQueries.query :=
+  let* verilog1' := Pass.pass_apply verilog_pipeline verilog1 in
+  let* verilog2' := Pass.pass_apply verilog_pipeline verilog2 in
+
+  let* inputs_eq := assert_dec (i2 = i1) "Incompatible inputs" in
+  let* outputs_eq := assert_dec (o2 = o1) "Incompatible outputs" in
+
+  VerilogEquivalence.equivalence_query verilog1' (rew_interface inputs_eq outputs_eq verilog2').
 
 (****** Continue here **********)
 
@@ -179,7 +187,7 @@ From Stdlib Require Import Structures.Equalities.
 From Stdlib Require Import Morphisms.
 From Stdlib Require Import Setoid.
 
-Lemma equivalence_query_clean_left v1 v2 smt :
+Lemma equivalence_query_clean_left {i o} (v1 v2 : vmodule i o) smt :
   VerilogEquivalence.equivalence_query v1 v2 = inr smt ->
   clean_module v1.
 Proof.
@@ -191,7 +199,7 @@ Proof.
   eassumption.
 Qed.
 
-Lemma equivalence_query_clean_right v1 v2 smt :
+Lemma equivalence_query_clean_right {i o} (v1 v2 : vmodule i o) smt :
   VerilogEquivalence.equivalence_query v1 v2 = inr smt ->
   clean_module v2.
 Proof.
@@ -205,71 +213,84 @@ Qed.
 
 Opaque verilog_pipeline.
 
-Theorem equivalence_query_general_unsat_correct v1 v2 smt :
+Theorem equivalence_query_general_unsat_correct {i o} (v1 : vmodule i o) (v2 : vmodule i o) smt :
   equivalence_query_general v1 v2 = inr smt ->
   (forall ρ, ~ satisfied_by ρ smt) ->
   v1 ~~ v2.
 Proof.
   unfold equivalence_query_general.
   intros. monad_inv.
+  rewrite rew_interface_refl in *.
   rewrite Pass.pass_correct with (v1:=v1) by eassumption.
   rewrite Pass.pass_correct with (v1:=v2) by eassumption.
   eapply VerilogEquivalenceCorrectness.equivalence_query_unsat_correct.
-  all: eassumption.
+  all: try eassumption.
 Qed.
 
-(* This only works because ~~~ (exact equivalence) says that internal
-   vars are the same. If it only matched external variables, then we
-   would need to have an existential here: valid executions of v1, v2
-   would have matching executions in v1', v2', but those would not be
-   definitionally equal. *)
-Lemma counterexample_transfer v1 v2 v1' v2' e1 e2 :
+Lemma transfer_execution {i o} (v v' : vmodule i o) e :
+  v ~~~ v' ->
+  v ⇓ e ->
+  exists e',
+    e =( LocationSet.of_varset (VarSet.of_list i) ∪ LocationSet.of_varset (VarSet.of_list o) )= e'
+    /\ v' ⇓ e'.
+Proof.
+  unfold "⇓", "~~~", module_locations.
+  intros Hequiv Hadmit.
+  exists (run_vmodule v' e).
+  unpack_goal.
+  - symmetry.
+    RegisterState.unpack_match_on.
+    + apply Facts.run_vmodule_preserve_inputs.
+    + rewrite <- Hequiv. assumption.
+  - setoid_rewrite Facts.run_vmodule_preserve_inputs at 2.
+    reflexivity.
+Qed.
+
+Lemma transfer_counterexample {i o} (v1 v1' v2 v2' : vmodule i o) e1 e2 :
   v1 ~~~ v1' ->
   v2 ~~~ v2' ->
-  counterexample_execution v1 e1 v2 e2 ->
-  counterexample_execution v1' e1 v2' e2.
+  counterexample_execution v1 v2 e1 e2 ->
+  exists e1' e2',
+    e1 =( LocationSet.of_varset (VarSet.of_list i) ∪ LocationSet.of_varset (VarSet.of_list o) )= e1'
+    /\ e2 =( LocationSet.of_varset (VarSet.of_list i) ∪ LocationSet.of_varset (VarSet.of_list o) )= e2'
+    /\ counterexample_execution v1' v2' e1' e2'.
 Proof.
   unfold counterexample_execution.
   intros Heq1 Heq2 [Hadmit1 [Hadmit2 [Hmatch_inputs Hmatch_outputs]]].
-  (* eexists. eexists. *)
+  destruct (transfer_execution v1 v1' e1) as [e1' [? ?]]; try assumption; expect 1.
+  destruct (transfer_execution v2 v2' e2) as [e2' [? ?]]; try assumption; expect 1.
+  exists e1'. exists e2'.
   unpack_goal.
-  - rewrite <- Heq1. apply Hadmit1.
-  - rewrite <- Heq2. apply Hadmit2.
-  - erewrite <- exact_equivalence_same_inputs by eassumption.
-    eassumption.
-  - erewrite <- exact_equivalence_same_outputs by eassumption.
-    eassumption.
+  - assumption.
+  - assumption.
+  - assumption.
+  - assumption.
+  - RegisterState.unpack_match_on.
+    do 2 match goal with
+    | H : _ =( ?l )= _ |- _ => (rewrite H || rewrite <- H); clear H
+    end.
+    assumption.
+  - RegisterState.unpack_match_on.
+    do 2 match goal with
+    | H : _ =( ?l )= _ |- _ => (rewrite H || rewrite <- H); clear H
+    end.
+    assumption.
 Qed.
 
-(* Proof using this rewrite only works because all of our
-   verilog-to-verilog passes (sort, simplify) preserve internal variables
-   exactly. If any of them added/removed vars, then we would need a
-   more relaxed equivalence, and that would not transfer counter-examples
-   exactly. The transferring would involve existentials (if there is a
-   counter-example for one module then there is one for the other, and the
-   two match on external ports)*)
-
-Global Instance Proper_counterexample_execution_exact_equivalence :
-  Proper
-    (exact_equivalence ==> eq ==> exact_equivalence ==> eq ==> iff)
-    counterexample_execution.
-Proof.
-  repeat intro; subst; split; intro.
-  - eapply counterexample_transfer; eauto.
-  - eapply counterexample_transfer; (symmetry + idtac); eauto.
-Qed.
-
-Theorem equivalence_query_general_sat_correct v1 v2 smt ρ :
+Theorem equivalence_query_general_sat_correct {i o} (v1 v2 : vmodule i o) smt ρ :
   equivalence_query_general v1 v2 = inr smt ->
   satisfied_by ρ smt ->
-  exists e1 e2, counterexample_execution v1 e1 v2 e2.
+  exists e1 e2, counterexample_execution v1 v2 e1 e2.
 Proof.
   intros. unfold equivalence_query_general in *. monad_inv.
-  eexists. eexists.
-  eapply counterexample_transfer with (v1:=v) (v2:=v0).
+  rewrite rew_interface_refl in *.
+  rename_match (ρ ⊧ smt) into Hsat.
+  eapply equivalence_query_sat_correct in Hsat; try eassumption; expect 1.
+  edestruct (transfer_counterexample v v1 v0 v2) as [e1' [e2' [? [? Hcex]]]].
   - symmetry. eapply Pass.pass_correct. eassumption.
   - symmetry. eapply Pass.pass_correct. eassumption.
-  - eapply equivalence_query_sat_correct. all: eassumption.
+  - eassumption.
+  - exists e1'. exists e2'. exact Hcex.
 Qed.
 
 Print Assumptions equivalence_query_general_unsat_correct.
