vera/VerilogEquivalence.v
@@ -57,23 +57,22 @@ Equations mk_outputs_distinct (inputs : list Var.t) : SMTLib.term SMTLib.Sort_Bo
   | (var :: vars) => SMTLib.Term_Or (mk_var_distinct var) (mk_outputs_distinct vars)
 }.
 
-Program Definition equivalence_query (verilog1 verilog2 : Verilog.vmodule) : string + SMTQueries.query :=
+Definition equivalence_query {i o} (verilog1 verilog2 : Verilog.vmodule i o) : string + SMTQueries.query :=
   trace "Construct equivalence query" (
-    let* inputs_ok1 :=
-      assert_dec
-        (Verilog.module_inputs verilog1 = Verilog.module_inputs verilog2)
-        ("Inputs don't match:" ++ newline
-        ++ to_string (Verilog.module_inputs verilog1) ++ newline
-        ++ to_string (Verilog.module_inputs verilog2) )
-      in
-    let* outputs_ok1 :=
-      assert_dec
-        (Verilog.module_outputs verilog1 = Verilog.module_outputs verilog2)
-        ("Outputs don't match:" ++ newline
-        ++ to_string (Verilog.module_outputs verilog1) ++ newline
-        ++ to_string (Verilog.module_outputs verilog2) )
-      in
-
+    (* let* inputs_ok1 :=
+     *   assert_dec
+     *     (Verilog.module_inputs verilog1 = Verilog.module_inputs verilog2)
+     *     ("Inputs don't match:" ++ newline
+     *     ++ to_string (Verilog.module_inputs verilog1) ++ newline
+     *     ++ to_string (Verilog.module_inputs verilog2) )
+     *   in
+     * let* outputs_ok1 :=
+     *   assert_dec
+     *     (Verilog.module_outputs verilog1 = Verilog.module_outputs verilog2)
+     *     ("Outputs don't match:" ++ newline
+     *     ++ to_string (Verilog.module_outputs verilog1) ++ newline
+     *     ++ to_string (Verilog.module_outputs verilog2) )
+     *   in *)
     let* smt1 := VerilogToSMT.verilog_to_smt VerilogLeft verilog1 in
     let* smt2 := VerilogToSMT.verilog_to_smt VerilogRight verilog2 in
 
